1084, 1093-1096, 1153-1156, 1160-1165, 1171-1173, 1180-1183
1084.2$$\begin{align*}
C(5;-3;7), r=2\\
(x-5)^{2}+(y+3)^{2}+(z-7)^{2}=4
\end{align*}$$
1093.2$$\begin{align*}
(x+14)^{2}+(y-11)^{2}+(z+12)^{2}=625\\
A(2;-1;3)\\
16^{2}+(-12)^{2}+15^{2}=256+144+225=625\text{ - на поверхности}
\end{align*}$$
1094.а$$\begin{align*}
A(-2;6;-3),x^{2}+y^{2}+z^{2}=4\\
(-2)^{2}+6^{2}+(-3)^{2}=4+36+9=49\\
\text{расстояние - }\sqrt{49}-\sqrt{4}=7-2=5
\end{align*}$$
1095.1$$\begin{align*}
z=3, x^{2}+y^{2}+z^{2}-6x+2y-10z+22=0\\
(x-3)^{2}+(y+1)^{2}+(z-5)^{2}=13
\end{align*}$$
1153$$\begin{align*}
x-2=0, \frac{x^{2}}{16}+\frac{y^{2}}{12}+\frac{z^{2}}{4}=1\\
\begin{cases}
x-2=0\\
\frac{x^{2}}{16}+\frac{y^{2}}{12}+\frac{z^{2}}{4}=1
\end{cases}\\
\frac{y^{2}}{12}+\frac{z^{2}}{4}=\frac{3}{4}\\
\frac{y^{2}}{9}+\frac{z^{2}}{3}=1\\
b=3,c=\sqrt{3}
\end{align*}$$1160$$\begin{align*}
x+mz-1=0, x^{2}+y^{2}-z^{2}=-1\\
\begin{cases}
x+mz-1=0\\
x^{2}+y^{2}-z^{2}=-1
\end{cases}\\
(1-mz)^{2}+y^{2}-z^{2}=-1\\
1-2mz+(mz)^{2}+y^{2}-z^{2}=-1\\
y^{2}-2mz+(m^{2}-1)z^{2}=-2\\
\begin{vmatrix}1&0\\
0&m^{2}-1\end{vmatrix}=m^{2}-1
\end{align*}$$
1180.1$$\begin{align*}
\begin{cases}
\frac{x^{2}}{81}+\frac{y^{2}}{36}+\frac{z^{2}}{9}=1\\
\frac{x-3}{3}=\frac{y-4}{-6}=\frac{z+2}{4}
\end{cases}\\
\begin{cases}
x=3t+3\\
y=-6t+4\\
z=4t-2
\end{cases}\\
\frac{(3t+3)^{2}}{81}+\frac{(-6t+4)^{2}}{36}+\frac{(4t-2)^{2}}{9}=1\\
\frac{9t^{2}+18t+9}{81}+\frac{36t^{2}-48t+16}{36}+\frac{16t^{2}-16t+4}{9}=1\\
t^{2}+2t+1+9t^{2}-12t+4+16t^{2}-16t+4=9\\
26t^{2}-26t
\end{align*}$$