101-110, 112, 113, 118, 119, 122-124, 136, 137, 143-146
101.$$\begin{align*}
(2+3i)(4-5i)+(2-3i)(4+5i)=\\
8-10i+12i-15i^{2}+8-12i+10i-15i^2=\\
46
\end{align*}$$
102.$$\begin{align*}
(x-1-i)(x-1+i)(x+1+i)(x+1-i)=\\
((x-1)^{2}-i^{2})((x+1)^{2}-i^{2})=\\
(x^{2}-2x+2)(x^{2}+2x+2)=\\
x^{4}+2x^{3}+2x^{2}-2x^{3}-4x^{2}-4x+2x^2+4x+4=\\
x^{4}+4
\end{align*}$$
103.$$\begin{align*}
(1+2i)x+(3-5i)y=1-3i\\
x+2xi+3y-5iy=1-3i\\
x+3y+(2x-5y)i=1-3i\\
\begin{cases}
x+3y=1:*2\\
2x-5y=3
\end{cases}\\
\begin{cases}
2x+6y=2\\
2x-5y=3
\end{cases}\\
11y=-1\implies y=-\frac{1}{11}\\
x-\frac{3}{11}=1\\
x=\frac{14}{11}
\end{align*}$$
104.
$$\begin {align*}
(1+i)x+(1+2i)y+(1+3i)z+(1+4i)t=1+5i\\
(3-i)x+(4-2i) Как ты это делаешь мне лень, писать научись:()
\end {align*}$$
105.а)$$\begin{align*}
(1+2i)^{6}=1^{6}+12i+15*4i^{2}+20*8i^{3}+15*16i^{4}+6*32i^{5}+64i^{6}=\\
1+12i-60-160i+240+192i-64=44i+117
\end{align*}$$
106.$$\begin{align*}
(x+yi)(z+wi)=mi\\
xz+xwi+yzi-wy=mi\\
\begin{cases}
xz-wy=0\\
xwi+yzi=mi
\end{cases}
\end{align*}$$
107.a)$$\begin{align*}
\frac{1+i\tan{\alpha}}{1-i\tan{\alpha}}=\frac{1+i\tan{\alpha}}{1-i\tan{\alpha}}\frac{1+i\tan{\alpha}}{1+i\tan{\alpha}}=\\
\frac{(1+i\tan{\alpha})^{2}}{1^{2}-(i\tan{\alpha})^{2}}=\frac{1+2i\tan{\alpha}+(i\tan{\alpha})^{2}}{1-i^{2}\tan^{2}{\alpha}}=\\
\frac{1-\tan^{2}{\alpha}+2i\tan{\alpha}}{1+\tan^{2}{\alpha}}=\cos^{2}{\alpha}-\sin^{2}{\alpha}+2i\cos{\alpha}
\end{align*}$$
108. a)$$\begin{align*}
\begin{cases}
(3-i)x+(4+2i)y=2+6i\\
(4+2i)x-(2+3i)y=5+4i
\end{cases}\implies\\
\begin{cases}
3x+4y+2iy-xi=2+6i\\
4x-2y+3iy+2ix=5+4i
\end{cases}\implies\\
\begin{cases}
3x+4y=2\\
2y-x=6\\
4x-2y=5\\
3y-2x=4
\end{cases}\\
3x=11\\
\end{align*}$$
109. а)
$$\begin{align*}
(\frac{-1}{2}+\frac{i \sqrt{3}}{2})^{2}=
\end{align*}$$
136. a)
$$\begin{align*}
(1+i \sqrt{3})(1+i)(\cos{\phi}+i\sin{\phi})=(1+i(\sqrt{3}+1)-\sqrt{3})(\cos{\phi}+i\sin{\phi})=\\
=\cos{\phi}-\cos{\phi}\sqrt{3}-\sin{\phi}(\sqrt{3}+1)-\sin{\phi}\sqrt{3}+i(\cos{\phi}(\sqrt{3}+1)+\sin{\phi})=\\
=\cos{\phi}(1-\sqrt{3})-\sin{\phi}(2\sqrt{3}+1)+i(\cos{\phi}(\sqrt{3}+1)+\sin{\phi})
\end{align*}$$
