---
date: 2023-09-29
tags:
  - homework
  - differential_equations
---
# ИДЗ
1. $xydx=(x^{2}-y^{2})dy$
   $xy=(x^{2}-y^{2})\frac{dy}{dx}\;|:x\neq0$
   $\frac{y}{x}=(1-(\frac{y}{x})^{2})\frac{dy}{dx}$
   $t=\frac{y}{x}\quad y=tx\quad dy=xdt+tdx$
   $\frac{dy}{dx}=x\frac{dt}{dx}+t$
   $t=(1-t^{2})(xt'+t)$
   $t=xt'-t^{2}xt'+t-t^{3}$
   $xt'(t^{2}-1)=t$
   $\frac{dt}{dx}=\frac{t}{x(t^{2}-1)}$
   $\frac{(t^{2}-1)dt}{t}=\frac{dx}{x}$
   $tdt-\frac{dt}{t}=\frac{dx}{x}$
   $\frac{1}{2}t^{2}-\ln{|t|}=\ln{|x|}$
   $\frac{e^{\frac{y^{2}}{2x^{2}}}}{y}=1$
   $y=e^{\frac{y^{2}}{2x^{2}}}$
   
1. $(x-1)y'+3x+2y+3=0$
   $(x-1)dy+(3x+2y+3)dx=0$
   $xdy-dy+3xdx+2ydx+3dx=0$
   $2d(xy)-dy+d(x^{2})+3dx=0$
   $d(2xy-y+x^{2}+3x)=0$
   $x^{2}+2xy+3x+y=C$
   $y=\frac{\tilde{C}+x^{2}+3x}{2x+1}$

1. $(4x^{2}+y^{4})dy-2xydx=0$
   $y=z^{m}\quad dy=mz^{m-1}dz$
   $(4x^{2}+z^{4m})mz^{m-1}dz=2xz^{m}dx$
   $2+m-1=4m+m-1=m+1$
   $2-1=4m-1=1$
   $4m=2\quad m=\frac{1}{2}$
   $\frac{4x^{2}+z^{2}}{2}z^{-\frac{1}{2}}dz=2xz^{\frac{1}{2}}dx$
   $z=xt\quad dz=xdt+tdx$
   $\frac{4x^{2}+x^{2}t^{2}}{2\sqrt{xt}}(t'+t)=2x\sqrt{xt}$
   $t'=\frac{4x^{2}t}{4x^{2}+x^{2}t^{2}}-t$
   $t'=\frac{4t}{4+t^{2}}-\frac{t4+t^{3}}{4+t^{2}}$
   $t'=-\frac{t^{3}}{4+t^{2}}$
   $dx=-\frac{4+t^{2}}{t^{3}}dt$
   $dx=-\frac{dt}{t}-\frac{4}{t^{3}}dt$
   $x=-\ln{t}+2t^{-2}$
   $t=\frac{z}{x}=\frac{y^{2}}{x}$
   $x=-\ln{\frac{y^{2}}{x}}+\frac{2x^{2}}{y^{4}}$
   $\frac{y^{2}}{x}=e^{\frac{2x^{2}}{y^{4}}-x}$
   $y=\sqrt{xe^{\frac{2x^{2}}{y^{4}}-x}}$
