---
date: 17.09.2023
tags:
  - homework
  - differential_equations
---

> [!NOTE] Задание 103
> $(y^{2}-2xy)dx+x^{2}dy=0$
> $y=zx,\quad dy=xdz+zdx$
> $(z^{2}x^{2}-2zx^{2})dx+(x^2)(xdz+zdx)=0$
> $x^{2}((z^{2}-2z)dx+(xdz+zdx))=0$
> $x^{2}=0\quad (z^{2}-z)dx+xdz=0$
> $\frac{dx}{x}+\frac{dz}{z^{2}-z}=0$
> $\int{\frac{dx}{x}}+\int{\frac{dz}{z^{2}-z}}=C$
> $\frac{1}{z(z-1)}=\frac{A}{z}+\frac{B}{z-1}$
> $1=A(z-1)+Bz$
> $1=-A\quad A=-1$
> $B=1$
> $\ln{|x|}+\ln{|z|}+\ln{|z-1|}=\ln{|C|}$
> $y(\frac{y}{x}-1)=C$
> Ответ:
> $y(\frac{y}{x}-1)=C$
> $x=0$

> [!NOTE] Задание 111
> $(y+\sqrt{xy})dx=xdy$
> $y=zx\quad dy=xdz+zdx$
> $(zx+x \sqrt{z})dx=x(xdz+zdx)$
> $x \sqrt{z}dx=x^{2}dz$
> $\frac{dx}{x}=\frac{dz}{\sqrt{z}}$
> $\ln{|x|}=2\sqrt{\frac{y}{x}}+C$

## ИДЗ

> [!NOTE] 1
> $x^{2}(x^{2}+4)y'=\cos^{2}{y}$
> $x^{2}(x^{2}+4)\frac{dy}{dx}=\cos^{2}{y}$
> $\frac{dx}{x^{2}(x^{2}+4)}=\frac{dy}{\cos^{2}{y}}$
> $x^{2}=t$
> $\frac{1}{t(t+4)}=\frac{A}{t}+\frac{B}{t+4}$
> $1=A(t+4)+Bt$
> $A=\frac{1}{4}\quad B=-\frac{1}{4}$
> $\frac{1}{4}\int{\frac{dx}{x^{2}}}+\frac{1}{4}\int{\frac{dx}{x^{2}+4}}=\frac{dy}{\cos^{2}{y}}$
> $-\frac{1}{4x}+\frac{1}{8}\arctan{\frac{x}{2}}=\tan{y}+C$

> [!NOTE] 2
> $(y-3x+2)dx+(3x-y-1)dy=0$
> $3x-y-1 = -1(y-3x+1)$
> $(y-3x+1)(dx-dy)+dx=0\;|:dx$
> $(y-3x+1)(1-(\frac{dy}{dx}))=-1$
> $\frac{dy}{dx}=\frac{y-3x+2}{y-3x+1}$
> $y-3x=z\quad y=z+3x\quad dy=dz+3dx$
> $\frac{dz}{dx}+3=\frac{z+2}{z+1}$
> $\frac{dz}{dx}+2=\frac{1}{z+1}$
> $dx=\frac{(z+1+\frac{1}{2}-\frac{1}{2})dz}{-2(z+1)+1}$
> $dx=(1+\frac{1}{-z-\frac{1}{2}})dz$
> $x=z-\ln{|z+\frac{1}{2}|}$
> $e^{x}=\frac{y-3x}{y-3x-\frac{1}{2}}$
> 
 
> [!NOTE] 3
> $y'+3y^{2}=3y,\quad y(0)=\frac{1}{2}$
> $\frac{dy}{dx}=3y-3y^{2}\;|:dy$
> $dx=\frac{dy}{3y-3y^{2}}$
> $\frac{1}{3y-3y^{2}}=\frac{A}{y}+\frac{B}{3-3y}$
> $A=\frac{1}{3}\quad B=1$
> $x=\ln{|y|}+\frac{1}{3}\ln{|1-y|}+C$
> $e^{3x}=Cy(1-y)$
> $C=4e^{0}=4$
> Ответ:
> $e^{3x}=Cy(1-y)$
