# ИДЗ 5

> [!NOTE] 1
> $$\begin{align*}
(y-3x^{2}y^{3})dx-(x+x^{3}y^{2})dy=0&\quad(1)\\
(1-x^{2}y^{2}-2x^{2}y^{2})ydx-(1-x^{2}y^{2}+2x^{2}y^{2})xdy=0\\
(1-x^{2}y^{2})(ydx-xdy)-(2x^{2}y^{2})dxy=0\\
dxy-d\frac{(xy)^{3}}{3}-2xdy+2(xy)^{2}xdy-d\frac{2}{3}(xy)^{3}=0\\
d(xy-\frac{(xy)^{3}}{3}-\frac{2}{3}(xy)^{3})-2(1-(xy)^{2})xdy=0\\
d(xy(1-(xy)^{2}))-2(1-(xy)^{2})xdy=0\;|:xy(1-(xy)^{2})\\
d\ln{xy(1-(xy)^{2})}-d2\ln{y}=0\\
\ln{xy(1-(xy)^{2})}-2\ln{y}=\ln{C}\\
y=\sqrt{\frac{xy(1-(xy)^{2})}{C}}
\end{align*}$$


> [!NOTE] 2
> $$\begin{align*}
x^{2}y^{3}dx+(x^{3}y^{2}+x)dy=0\\
x^{2}y^{2}ydx+(x^{2}y^{2}+1)xdy=0\\
x^{2}y^{2}dxy+xdy=0\\
d\frac{x^{3}y^{3}}{3}+xdy=0\;|:xy\\
(xy)^{-1}d\frac{1}{3}x^{3}y^{3}+\frac{dy}{y}=0\\
d\frac{(xy)^{4}}{4}+d\ln{y}=0\\
d(\frac{(xy)^{4}}{4}+\ln{y})=0\\
\frac{(xy)^{4}}{4}+\ln{y}=C
\end{align*}$$
