---
date: 2023-10-06
tags:
  - practice
  - differential_equations
---
$(x_{0},y_{0})$
$f(y)dy=p(x)dx$
$\int\limits_{y_{0}}^{y}{f(y)dy}=\int\limits_{x_{0}}^{x}{p(x)dx}$
$F(y)-F(y_{0})=G(x)-G(x_{0})$

# Уравнение Бернулли
$y'+a(x)y=b(x)y^{n}$
$z=y^{1-n}$

> [!note]
> $y'+2y=e^{x}y^{2}$
> $\frac{y'}{y^{2}}+\frac{2}{y}=e^{x}$
> $z=\frac{1}{y}$
> $-(\frac{1}{y})'+2(\frac{1}{y})=e^{x}$
> $z=\frac{1}{y}$
> $-z'+2z=e^{x}$
> $-z'+2z=0$
> $\frac{dz}{dx}=2z$
> $\ln{z}=2x+C$
> $z=e^{2x}C$
> $C=C(x)$
> $z=e^{2x}C(x)$
> $z'=2e^{2x}C(x)+e^{2x}C'(x)$
> $-2e^{2x}C(x)+e^{2x}C'(x)+2C(x)e^{2x}=e^{x}$
> $C'(x)=e^{x}$
> $C(x)=-e^{-x}+D$
> $z(x)=e^{2x}(-e^{-x}+D)$
> $y=\frac{1}{z}=\frac{1}{e^{2x}(-e^{-x}+D)}$

153, 154

> [!NOTE] 153
> $y'=y^{4}\cos{x}+y \tan{x}$
> $z=y^{-3}\quad z'=-3y^{-4}y'$
> $-\frac{z'}{3}=\cos{x}+z \tan{x}$
> $z'=-3z \tan{x}$
> $\frac{dz}{z}=-3\tan{x}\;dx$
> $\ln{z}=-3\int{\frac{\sin{x}}{\cos{x}}}dx+C$
> $t=\cos{x}\quad dt=-\sin{x}dx$
> $\ln{z}=3\ln{t}+C$
> $z=C\cos^{3}{x}$
> $z'=3\sin{x}\cos^{2}{x}C(x)+C'(x)\cos^{3}{x}$
> $-\frac{3\sin{x}\cos^{2}{x}C(x)+C'(x)\cos^{3}{x}}{3}=\cos{x}+C \cos^{3}{x}\tan{x}$
> $\frac{C'(x)\cos^{3}{x}}{3}=\cos{x}$
> $C'(x)=-\frac{3}{\cos^{2}{x}}$
> $C(x)=-3\tan{x}+D$
> $\frac{1}{y^{3}}=\cos^{3}{x}(-3\tan{x}+D)$

# Уравнение Рикатти
$y'+a(x)y+b(x)y^{2}=c(x)$
Сводится к уравнению Бернулли с заменой $y=z(x)+y_{1}(x)$, где $y_1$ - частное решение.


> [!NOTE] 167
> $x^{2}y'+xy+x^{2}y^{2}=4$
> $y'-\frac{y}{x}+y^{2}=\frac{4}{x^{2}}$
> $y_{1}=\frac{a}{x}\quad y_{1}'=-\frac{a}{x^{2}}$
> $-\frac{a}{x}+\frac{a}{x^{2}}+\frac{a^{2}}{^{2}}=\frac{4}{x^{2}}$
> $\frac{a^{2}}{x^{2}}=\frac{4}{x^{2}}\quad a=\pm2$
> $y=z(x)+\frac{2}{x}$
> $y'=z'(x)-\frac{2}{x^{2}}$
> $z'-\frac{2}{x^{2}}+\frac{1}{x}(z+\frac{2}{x})+(z+\frac{2}{x})=\frac{4}{x^{2}}$
> $z'+\frac{z}{x}+z^{2}+\frac{4z}{x}+\frac{4}{x^{2}}=\frac{4}{x^{2}}$
> $z'+\frac{5z}{x}=-z^{2}$ - уравнение Бернулли
> $z=0$ - решение
> $\frac{z'}{z^{2}}+\frac{5}{xz}=-1$
> $t(x)=\frac{1}{z(x)}\quad z'=\frac{1}{t^{2}(x)}t'$
> $-t'(x)=\frac{5t(x)}{x}=-1$
> $t'=\frac{5t}{x}$