---
date: 18.11.2023
tags:
  - homework
  - differential_equations
---
# ИДЗ 3
![[photo_2023-11-18_17-14-23.jpg]]
![[photo_2023-11-18_17-14-22.jpg]]

# ИДЗ 4

> [!NOTE] 1
> $$\begin{align*}
xy'=y^{2}+2(x+1)y+x^{2}+x\\
y'-\frac{2(x+1)y}{x}-\frac{y^{2}}{x}=x+1\\
y_{1}=ax\quad \frac{dy_{1}}{dx}=a\\
a-2a(x+1)-a^{2}x=x+1\\
(a^{2}+2a+1)x=a-1-2
---
y_{1}=-x\\
y=-x+z\quad dy=-dx+dz\\
-1+z'-\frac{2(x+1)(z-x)}{x}-\frac{(z-x)^{2}}{x}=x+1\\
\frac{dz}{dx}=\frac{2(x+1)(z-x)}{x}+\frac{(z-x)^{2}}{x}+x+1+1\\
\frac{dz}{dx}=\frac{2zx+2z-2x^{2}-2x+z^{2}-2zx+x^{2}}{x}+x+2\\
\frac{dz}{dx}=\frac{z(z-2)-x(x-2)}{x}+x+2\\
\frac{dz}{dx}=\frac{z(z-2)}{x}+4\\
\frac{dz}{dx}=\frac{z(z-2)}{x}\\
\frac{dz}{z(z-2)}=\frac{dx}{x}\\
-\frac{dz}{2z}+\frac{dz}{2(z-2)}=\frac{dx}{x}\\
-\frac{1}{2}\ln{z}+\frac{1}{2}\ln{z-2}=\ln{x}\\
\frac{\sqrt{z-2}}{\sqrt{z}}=x\\
z=y+x\\
\frac{\sqrt{y+x-2}}{\sqrt{y+x}}=x\\
\end{align*}$$

> [!NOTE] 2
> $$\begin{align*}
((x-y)^{2}-x)dx+(y-(x-y)^{2})dy=0\\
(x-y)^{2}dx-xdx+ydy-(x-y)^{2}dy=0\\
(x-y)^{2}d(x-y)-xdx+ydy=0\\
\frac{1}{3}(x-y)^{3}-\ln{x}+\ln{y}=0\\
y=\frac{x}{e^{\frac{1}{3}(x-y)^{3}}}
\end{align*}$$
