---
date: 27.10.2023
tags:
  - practice
  - differential_equations
---
## Интегрирующий множитель
$P(x,y)dx+Q(x,y)dy=0$
$P'_{y}\neq Q'_{x}$
$\mu(x,y)P(x,y)dx+\mu(x,y)Q(x,y)dy=0$
$\mu'_{y}P+\mu P'_{y}=\mu'_{x}Q+\mu Q'_{x}$
$\mu'_{x}Q+\mu'_{y}P=(P'_{y}+Q'_{x})\mu$
Выбираем, от чего будет зависеть $\mu$
1. $\mu=\mu(x)$
2. $\mu=\mu(y)$

## Группировка дифференциалов
1. $x^{n}dx=\frac{1}{n+1}dx^{n+1}$
2. $d(x+y)=dx+dy$
3. $d(xy)=ydx+xdy$
4. $d(\frac{x}{y})=\frac{ydx-xdy}{y^{2}}$

# Примеры
> [!NOTE] 195
> Интегрирующий множитель
> $(x^{2}+y^{2}+x)dx+ydy=0$
> $P'_{y}=2y\quad Q'_{x}=0$
> $y\mu'_{x}+(x^{2}+y^{2}+x)\mu'_{y}=2y\mu$
> 
> Пусть $\mu=\mu(x)$
> $y\mu'=2y\mu(x)$
> $\frac{d\mu}{dx}=2\mu$
> $\ln{|\mu|}=2x$
> $\mu(x)=e^{2x}$
> 
> $(x^{2}+y^{2}+x)e^{2x}dx+ye^{2x}dy=0$
> $F=\int{P}dx=\int{(x^{2}+x)e^{2}}dx+y^{2}\int{e^{2x}}dx$
> $\int{udv}=uv-\int{vdu}$
> $F=y^{2}(\frac{1}{2})e^{2x}+(\frac{1}{2})\int{(x^{2}+x)de^{2x}}$
> $\int{(x^{2}+x)de^{2x}}=(x^{2}+x)e^{2x}-\int{e^{2x}d(x^{2}+x)}=(x^{2}+x)e^{2x}-2\int{xe^{2x}dx}-\int{e^{2x}dx}=$
> $=(x^{2}+x)e^{2}-\frac{1}{2}e^{2x}-\int{xde^{2x}}=(x^{2}+x-\frac{1}{2})e^{2x}-xe^{2x}+\int{e^{2x}dx}+C=x^{2}e^{2x}+C$
> $F=\frac{1}{2}(y^{2}+x^{2})e^{2x}+C=0$
> 
> ---
> Группировка дифференциалов
> $(x^{2}+y^{2}+x)dx+ydy=0$
> $(x^{2}+y^{2})dx+xdx+ydy=0$
> $(x^{2}+y^{2})dx+\frac{1}{2}dx^{2}+\frac{1}{2}dy^{2}=0$
> $(x^{2}+y^{2})dx+\frac{1}{2}d(x^{2}+y^{2})=0 | \cdot\frac{2}{x^{2}+y^{2}}$
> $2dx+\frac{d(x^{2}+y^{2})}{x^{2}+y^{2}}=0$
> $2dx+d\ln{|x^{2}+y^{2}|}=0$
> $d(2x+\ln{(x^{2}+y^{2})})=0$
> $2x+\ln{(x^{2}+y^{2})}=C$

> [!NOTE] 196
> $(x^{2}+y^{2}+y)dx-xdy=0$
> $P'_{y}=2y+1\quad Q'_{x}=-1$
> $-x\mu'_{x}-(x^{2}+y^{2}+y)\mu'_{y}=(2y+2)\mu$
> 
> $(x^{2}+y^{2})dx+\underbrace{ydx+xdy}=0$
> $(x^{2}+y^{2})dx+y^{2}d(\frac{x}{y})=0 |:y^{2}$
> $(\frac{x^{2}}{y^{2}}+1)dx+d(\frac{x}{y})=0$
> Есть два способа
> 1. Разделить на $\frac{x^{2}}{y^{2}}+1$
> 2. Ввести замену $t=\frac{x}{y}$
> 
> По первому
> $dx+\frac{d(\frac{x}{y})}{1+(\frac{x}{y})^{2}}=0$
> $dx+d\arctan{\frac{x}{y}}=0$
> $x+\arctan{\frac{x}{y}}=C$


197-204

> [!NOTE] 197
> $ydy=(xdy+ydx)\sqrt{1+y^{2}}$
> $ydy=d(xy)\sqrt{1+y^{2}}$
> $\frac{ydy}{\sqrt{1+y^{2}}}=dxy$
> $\frac{1}{2}\frac{dy^{2}}{\sqrt{1+y^{2}}}=dxy$
> $\frac{d(y^{2}+1)}{2\sqrt{y^{2}+1}}=dxy$
> $d(\sqrt{1+y^{2}})=dxy$
> $\sqrt{1+y^{2}}=xy+C$


> [!NOTE] 198
> $xy^{2}(xy'+y)=1$
> $xy^{2}(\frac{xdy}{dx}+y)=1$
> $x^{2}y^{2}dy+(xy^{3}-1)dx=0$
> $Q'_{x}=2x\quad P'_{y}=3y^{2}$
> $\mu'_{x}x^{2}y^{2}+\mu'_{y}(xy^{3}-1)=(3y^{2}+2x)\mu$
> 
> $\sqsupset \mu=\mu(y)$
> $xy^{3}\mu'_{x}=(3y^{2}+2x)\mu$
> 
> $\frac{x^{2}}{3}dy^{3}+\frac{y^{3}}{2}dx^{2}=0$
> $\frac{2dy^{3}}{y^{3}}+\frac{3dx^{2}}{x^{2}}=0$
> $2d\ln{|y^{3}|}+3d\ln{x^{2}}=0$
> $2\ln{|y^{3}|}+3\ln{x^{2}}=C$
> $y^{6}x^{6}=C$
> $x=0$ входит в решение


> [!NOTE] 199
> $y^{2}dx-(xy+x^{3})dy=0$
> $yydx-yxdy-x^3dy=0$
> $y^{3}d(\frac{x}{y})-x^{3}dy=0|:x^{3}$
> $\frac{d(\frac{x}{y})^{-2}}{-2}-dy=0$
> $-d(\frac{y^{2}}{2x^{2}}-y)=0$
> $-\frac{y^{2}}{2x^{2}}-y=C$


> [!NOTE] 200
> $(y-\frac{1}{x})dx+\frac{dy}{y}=0$
> $ydx-d\ln{|x|}+d\ln{|y|}=0$


