3235.$$\begin{align*}
u=x^{m}y^{n}\\
\frac{\delta u}{\delta x}=mx^{m-1}y^{n}\\
\frac{\delta u}{\delta y}=nx^{m}y^{n-1}\\
\frac{\delta u^{2}}{\delta x^{2}}=m(m-1)x^{m-2}y^{n}\\
\frac{\delta u^{2}}{\delta y^{2}}=n(n-1)x^{m}y^{n-2}\\
\frac{\delta u^{2}}{\delta x \delta y}=\frac{\delta u^{2}}{\delta y \delta x}=mnx^{m-1}y^{n-1}\\
du(x,y)=(mx^{m-1}y^{n})dx+(nx^{m}y^{n-1})dy\\
d^{2}u(x,y)=(m(m-1)x^{m-2}y^{n})dx^{2}+2(mnx^{m-1}y^{n-1})dxdy+(n(n-1)x^{m}y^{n-2})dy^{2}
\end{align*}$$
3256.$$\begin{align*}
u=x-y+x^{2}+2xy+y^{2}+x^{3}-3x^{2}y+x^{4}-4x^{2}y^{2}+y^{4}\\
\frac{\delta u^{4}}{\delta x^{4}}=4!\\
\frac{\delta u^{4}}{\delta x^{3}\delta y}=0\\
\frac{\delta u^{4}}{\delta x^{2}\delta y^{2}}=24-16=8
\end{align*}$$
3268.$$\begin{align*}
u=x^{4}-2x^{3}y-2xy^{3}+y^{4}+x^{3}-3x^{2}y-3xy^{2}+y^{3}+2x^{2}-xy+2y^{2}+x+y+1\\
\frac{\delta u^{4}}{\delta x^{4}}=4!=24\\
\frac{\delta u^{4}}{\delta x^{3}}=24x-12y+6\quad\frac{\delta u^{4}}{\delta x^{3}\delta y}=-12\\
\frac{\delta u^{4}}{\delta x^{2}}=12x^{2}-12xy+6x-6y+4\quad\frac{\delta u^{4}}{\delta x^{2}\delta y^{2}}=0\\
\frac{\delta u^{4}}{\delta x}=4x^{3}-6x^{2}y-2y^{3}+3x^{2}-6xy-3y^{2}+4x-y+1\\
\frac{\delta u^{4}}{\delta x\delta y^{3}}=-2(3!)=-12\\
\frac{\delta u^{4}}{\delta y^{4}}=4!=24\\
d^{4}u(x,y)=(24)dx^{4}+4(-12)dx^{3}dy+6(0)dx^{2}dy^{2}+4(-12)dydx^{3}+(24)dy^{4}
\end{align*}$$
3621.$$\begin{align*}
f(x,y)=z=x^{2}+(y-1)^{2}\\
f''_{xx}=2\\
f''_{yy}=2\\
f''_{xy}=0
\end{align*}$$