$$\begin{align*}
\frac{\delta u}{\delta y}&\quad\frac{\delta u}{\delta x}\\
\frac{\delta^2 u}{\delta y^2}&\quad\frac{\delta^2 u}{\delta x^2}\\
\frac{\delta^2 u}{\delta y\delta x}&\quad\frac{\delta^2 u}{\delta x\delta y}
\end{align*}$$
â„–3213-3228

3217. $$\begin{align*}
u=x\sin{x+y}\\
\frac{\delta u}{\delta y}=x(-\cos{x+y})\\
\frac{\delta u}{\delta x}=\sin{(x+y)}+x-\cos{(x+y)}\\
\frac{\delta^2 u}{\delta y^2}=x(-\sin{x+y})\\
\frac{\delta^2 u}{\delta x^2}=-2\cos{(x+y)}+x(-\sin{(x+y)})\\
\frac{\delta^2 u}{\delta x\delta y}=-\cos{(x+y)}+x(-\sin{(x+y)})\\
\frac{\delta^2 u}{\delta y\delta x}=-\cos{(x+y)}+x(-\sin{(x+y)})
\end{align*}$$

3213. $$\begin{align*}
u=x^{4}+y^{4}-4x^{2}y^{2}\\
\frac{\delta u}{\delta y}=4y^{3}-8x^{2}y\\
\frac{\delta u}{\delta x}=4x^{3}-8xy^{2}\\
\frac{\delta^{2} u}{\delta y^{2}}=12y^{2}-8x^{2}\\
\frac{\delta^{2} u}{\delta x^{2}}=12x^{2}-8y^{2}\\
\frac{\delta^{2} u}{\delta x\delta y}=-16xy\\
\frac{\delta^{2} u}{\delta y\delta x}=-16xy
\end{align*}$$
3214. $$\begin{align*}
u=xy+\frac{x}{y}\\
\frac{\delta u}{\delta y}=x-\frac{x}{y^{2}}\\
\frac{\delta u}{\delta x}=y+\frac{1}{y}\\
\frac{\delta^{2} u}{\delta y^{2}}=2\frac{x}{y^{3}}\\
\frac{\delta^{2} u}{\delta x^{2}}=0\\
\frac{\delta^{2} u}{\delta x\delta y}=1-\frac{1}{y^{2}}\\
\frac{\delta^{2} u}{\delta y\delta x}=1-\frac{1}{y^{2}}
\end{align*}$$

3216. $$\begin{align*}
u=\frac{x}{\sqrt{x^{2}+y^{2}}}=f(x)g(h(x)+j(y))\\
\frac{\delta u}{\delta y}=-\frac{1}{2}x(x^{2}+y^{2})^{-\frac{3}{2}}2y\\
\frac{\delta u}{\delta x}=(x^{2}+y^{2})^{-\frac{1}{2}}-\frac{1}{2}(x^{2}+y^{2})^{-\frac{3}{2}}2x\\
\frac{\delta^2 u}{\delta y^{2}}=-x(2(x^{2}+y^{2})^{-\frac{3}{2}}-6y^{2}(x^{2}+y^{2})^{-\frac{5}{2}})\\
\frac{\delta^{2} u}{\delta x^{2}}=-\frac{1}{2}2x(x^{2}+y^{2})^{-\frac{3}{2}}-\frac{1}{2}(2(x^{2}+y^{2})^{-\frac{3}{2}}-6x(x^{2}+y^{2})^{-\frac{5}{2}})\\
\frac{\delta^{2} u}{\delta x\delta y}=-y(x^{2}+y^{2})^{-\frac{3}{2}}+3xy(x^{2}+y^{2})^{-\frac{5}{2}}\\
\frac{\delta^{2} u}{\delta y\delta x}=-y((x^{2}+y^{2})^{-\frac{3}{2}}-3x^{2}(x^{2}+y^{2})^{-\frac{5}{2}})
\end{align*}$$

3220. $$\begin{align*}
u=x^{yx}\\
\frac{\delta u}{\delta x}=y\frac{x^{yx}}{\ln{x}}\\
\frac{\delta u}{\delta y}=\frac{x^{xy}}{\ln{x}}\\
\frac{\delta^{2} u}{\delta y^{2}}=\frac{x^{xy}}{\ln^{2}{x}}\\
\frac{\delta^{2} u}{\delta x^{2}}=\\
\frac{\delta^{2} u}{\delta y\delta x}=\\
\frac{\delta^{2} u}{\delta x\delta y}=\frac{x^{yx}}{\ln{x}}+y\frac{x^{xy}}{\ln^{2}{x}}
\end{align*}$$

3594.$$\begin{align*}
f(x,y)=\ln{(1+x+y)}\\
f'_{x}=\frac{1}{x+1+y}\\
f'_{y}=\frac{1}{1+x+y}\\
f''_{xx}=-\frac{1}{(1+x+y)^{2}}\\
f''_{yy}=-\frac{1}{(1+x+y)^{2}}\\
f''_{xy}=-\frac{1}{(1+x+y)^{2}}\\
f''_{yx}=-\frac{1}{(1+x+y)^{2}}\\
f(x,y)=0+(x+y)+\frac{1}{2}(-x^{2}-2xy-y^{2})
\end{align*}$$
3595.$$\begin{align*}
f(x,y)=e^{x}\sin{y}\\
f_{x}'=e^{x}\sin{y}\\
f_{y}'=-e^{x}\cos{y}\\
f''_{xx}=e^{x}\sin{y}\\
f_{yy}''=-e^{x}\sin{y}\\
f_{xy}''=-e^{x}\cos{y}\\
f_{yx}''=-e^{x}\cos{y}\\
f(x,y)=0+(-y)+\frac{1}{2}(-2xy)
\end{align*}$$
3596.$$\begin{align*}
f(x,y)=e^{x}\cos{y}=1\\
f'_{x}=e^{x}\cos{y}=1\\
f'_{y}=e^{x}\sin{y}=0\\
f_{xx}''=e^{x}\cos{y}=1\\
f_{yy}''=-e^{x}\cos{y}=1\\
f_{xy}''=e^{x}\sin{y}=0\\
f_{yx}''=e^{x}\sin{y}=0\\
f(x,y)=1+(x)+\frac{1}{2}(x^{2}+y^{2})
\end{align*}$$
3597.$$\begin{align*}
f(x,y)=\sin{x}\sinh{y}\\
f'_{x}=-\cos{x}\sinh{y}\\
f'_{y}=\sin{x}\cosh{y}\\
f_{xx}''=-\sin{x}\sinh{y}\\
f_{yy}''=\sin{x}\sinh{y}\\
f_{xy}''=-\cos{x}\cosh{y}\\
f_{yx}''=-\cos{x}\cosh{y}\\
f(x,y)=\frac{1}{2}(x^{2}+y^{2})+o
\end{align*}$$
3599.$$\begin{align*}
f(x,y)=\sin{x^{2}+y^{2}}\\
f'_{x}=-\cos{x^{2}+y^{2}}2x\\
f'_{y}=-\cos{x^{2}+y^{2}}2y\\
f_{xx}''=-2x\sin{x^{2}+y^{2}}-2\cos{x^{2}+y^{2}}\\
f_{yy}''=-2y\sin{x^{2}+y^{2}}-2\cos{x^{2}+y^{2}}\\
f_{xy}''=-\sin{x^{2}+y^{2}}4xy\\
f_{yx}''=-\sin{x^{2}+y^{2}}4yx\\
f(x,y)=\frac{1}{2}(-2x^{2}-2y^{2})
\end{align*}$$
3600.$$\begin{align*}
f(x,y)=\ln(1+x)\ln(1+y)\\
f_{x}'=\frac{\ln{(1+y)}}{1+x}\\
f_{y}'=\frac{\ln{(1+x)}}{1+y}\\
f_{xx}''=
\end{align*}$$