# Иррациональные интегралы
1926-1933
$$\begin{align*}
\int{\frac{dx}{\sqrt{x}(x+3)}}\\
\sqrt{x}=t\quad x=t^{2}\\
\frac{dx}{2\sqrt{x}}=dt\\
\int{\frac{2dt}{t^{2}+3}}=\frac{2}{\sqrt{3}}\arctan{\frac{x}{\sqrt{3}}}+2C
\end{align*}$$
$$\begin{align*}
\int{\frac{\sqrt{x+2}}{x-3}dx}\\
\sqrt{x+2}=t\quad x=t^{2}-2\\
\frac{dx}{2\sqrt{x+2}}=dt\\
\int{\frac{2t^{2}dt}{t^{2}-5}}=\int{\frac{2(t^{2}-5)+10}{t^{2}-5}dt}=\int{2+\frac{10}{t^{2}-5}dt}=2x+4+\frac{10}{\sqrt{5}}\arctan{\frac{x+2}{\sqrt{5}}}+10C
\end{align*}$$
1873$$\begin{align*}
\int{\left(\frac{x}{x^{2}-3x+2}\right)^{2}dx}\\
\int{\frac{x^{2}}{(x-2)^{2}(x-1)^{2}}dx}\\
\frac{x^{2}}{(x-2)^{2}(x-1)^{2}}=\frac{A}{x-2}+\frac{B}{(x-2)^{2}}+\frac{C}{x-1}+\frac{D}{(x-1)^{2}}=\\
=\frac{A(x-2)(x-1)^{2}+B(x-1)^{2}+C(x-1)(x-2)^{2}+D(x-2)^{2}}{(x-1)^{2}(x-2)^{2}}\\
\begin{cases}
0=A+C\\
1=-4A-5C+D+B\\
0=5A+8C-2B-4D\\
0=-2A-4C+B+4D
\end{cases}\\
D=1\quad B=4\quad C=4\quad A=-4\\
-4\int{\frac{dx}{x-2}}+4\int{\frac{dx}{(x-2)^{2}}}+4\int{\frac{dx}{x-1}}+\int{\frac{dx}{(x-1)^{2}}}=\\
=-4\ln{x-2}-\frac{4}{x-2}+4\ln{x-1}-\frac{1}{x-1}+C\\
C=-4C_{1}+4C_{2}+4C_{3}+C_{4}
\end{align*}$$
1927$$\begin{align*}
\int{\frac{dx}{x(1+2\sqrt{x}+x^{\frac{1}{3}})}}\\
x=t^{6}\\
dx=6t^{5}dt\\
\int{\frac{6t^{5}dt}{t^{6}(1+2t^{3}+t^{2})}}=\int{\frac{6dt}{t(1+2t^{3}+t^{2})}}=6\int{\frac{dt}{t(t+1)(2t^{2}-t+1)}}\\
\frac{1}{t(t+1)(2t^{2}-t+1)}=\frac{A}{t}+\frac{B}{t+1}+\frac{Cx+D}{2t^{2}-t+1}
\end{align*}$$