1400. 
$$\begin{align*}
\lim\limits_{x\to+\infty}x^\frac{3}{2}(\sqrt{x+1}+\sqrt{x-1}-2\sqrt{x})\\\\
f(x)=\sum\limits_{k=0}^{n}\frac{f^{(k)}(a)}{k!}(x-a)^{k}+R_{n}(x)\\
f(x)=\sqrt{x+1}\\
f^{(k)}(0)=(-1)^{k+1}\frac{\frac{2k!}{2^{k-1}k!}}{2^{k}}\\
f(x)=\sum\limits_{k=0}^{n}\frac{(-1)^{k+1}\frac{2k!}{2^{2k-1}k!}}{k!}(x)^{k}+R_{n}(x)\\
\\
f(x)=\sqrt{x-1}\\
f^{(k)}(2)=(-1)^{k+1}\frac{2k!}{2^{2k-1}k!}\\
f(x)=\sum\limits_{k=0}^{n}\frac{(-1)^{k+1}\frac{2k!}{2^{2k-1}k!}}{k!}(x-2)^{k}+R_{n}(x)\\
\\
f(x)=\sqrt{x}\\
f^{(k)}(1)=(-1)^{k+1}\frac{2k!}{2^{2k-1}k!}\\
f(x)=\sum\limits_{k=0}^{n}\frac{(-1)^{k+1}\frac{2k!}{2^{2k-1}k!}}{k!}(x-1)^{k}+R_{n}(x)
\end{align*}$$
$n=3$
$$\begin{align*}
\sqrt{x+1}=1+\frac{x}{2}-\frac{x^2}{8}+\frac{3x^3}{16}+o(x^{3})\\
\sqrt{x-1}=1+\frac{x-2}{2}-\frac{(x-2)^{2}}{8}+\frac{3(x-2)^{3}}{16}+o(x^{3})\\
\sqrt{x}=1+\frac{x-1}{2}-\frac{(x-1)^{2}}{8}+\frac{3(x-1)^{3}}{16}+o(x^{3})\\
\\
\lim\limits_{x\to+\infty}x^{\frac{3}{2}}(\sqrt{x+1}+\sqrt{x-1}-2\sqrt{x})=\\
=\lim\limits_{x\to+\infty}x^{\frac{3}{2}}\left(3+\frac{3x-3}{2}-\frac{3x^{2}-6x+5}{8}+\frac{9x^{3}-9x^{2}+27x-9}{16}+o(x^{3})\right)=\\
=\lim\limits_{x\to+\infty}x^{\frac{3}{2}}\left(\frac{48+24x-24-6x^{2}+12x-10+9x^{3}-9x^{2}+27x-9}{16}+o(x^{3})\right)=\\
=\lim\limits_{x\to+\infty}x^{\frac{3}{2}}\left(\frac{9x^{3}-15x^{2}+63x+5}{16}+o(x^{3})\right)=\infty
\end{align*}$$
![[Pasted image 20230317181447.png]]
1405. 
$$\begin{align*}
\lim\limits_{x\to0}(\frac{1}{x}-\frac{1}{\sin{x}})\\
\sin{x}=\sum\limits_{k=0}^{n}\frac{(-1)^{k}x^{2k+1}}{(2k+1)!}+o(x^{2n+2})
\end{align*}$$$n=1$
$$\begin{align*}
\sin{x}=x+o(x)\\
\lim\limits_{x\to0}\left(\frac{1}{x}-\frac{1}{\sin{x}}\right)=\lim\limits_{x\to0}\left(\frac{1}{x}-\frac{1}{x}+o(x)\right)=0
\end{align*}$$
