$$\begin{align*}
\int{\left(\frac{7}{5x^{2}+2}-2\sin{3x}+3^{7x}\right)}dx\\
\int{\frac{7}{5x^{2}+2}}dx-2\int{\sin{3x}}dx+\int{3^{7x}}dx\\
\frac{1}{5}\int{\frac{7}{x^{2}+\frac{2}{5}}}dx-\frac{2\cos{x}}{3}+2C_{2}+\frac{3^{7x}}{7\ln{|3|}}+C_{3}\\
\frac{7}{5}\frac{1}{\sqrt{\frac{2}{5}}}\arctan{\frac{x}{\sqrt{\frac{2}{5}}}}+\frac{7}{5}C_{1}-\frac{2\cos{x}}{3}+2C_{2}+\frac{3^{7x}}{7\ln{|3|}}+C_{3}
\end{align*}$$
$$\begin{align*}
\int{(\frac{6}{\sqrt{4+x^{2}}}-\frac{3x+x^{3}}{x^{3}}+6x^{\frac{7}{5}})}\\
6\int{\frac{1}{\sqrt{4+x^{2}}}}dx-\int{\frac{3}{x^{2}}}dx-\int{1}dx+6\int{x^{\frac{7}{5}}}dx\\
6\int{\frac{1}{\sqrt{4+x^{2}}}}dx-3\left(-\frac{1}{x}+C_{2}\right)-(x+C_{3})+6\left(\frac{x^{5\frac{12}{5}}}{7}+C_{4}\right)\\
6(\ln{|x+\sqrt{x^{2}+4}|}+C_{1})-3\left(-\frac{1}{x}+C_{2}\right)-(x+C_{3})+6\left(\frac{x^{5\frac{12}{5}}}{7}+C_{4}\right)
\end{align*}$$
$$\begin{align*}
\int{\cos{4x+3}}dx\\
t=4x+3\\
dt=4dx\\
\int{\cos{t}}\frac{dx}{4}=\frac{1}{4}(\sin{t}+C)=\frac{1}{4}\sin{(4x+3)}+\frac{1}{4}C
\end{align*}$$
Не брать в замену корни, $e$, логарифмы и тригонометрию. Выражение не упростится.
$$\begin{align*}
\int{\frac{dx}{\sqrt{x^{2}+2x+7}}}\\
t=x+1\\
dt=dx\\
\int{\frac{dt}{\sqrt{t^{2}-8}}}\\
\ln{|t+\sqrt{t^{2}-8}|}+C\\
\ln{|x+1+\sqrt{x^{2}+2x+7}|}+C
\end{align*}$$
$$\begin{align*}
\int{((2x-1)\sin{(2x)})}dx\\
u=2x-1\\
du=2dx\\
dv=\sin{2x}dx\\
v=-\frac{1}{2}\cos{2x}\\
\int{udv}=uv-\int{vdu}\\
(2x-1)(-\frac{1}{2}\cos{2x})+\int{\cos{2x}dx}\\
(2x-1)(-\frac{1}{2}\cos{2x})+\frac{1}{2}\sin{2x}+C
\end{align*}$$
$$\begin{align*}
\int{\arctan{x}}\:dx\\
u=\arctan{x}\\
du=\frac{1}{1+x^{2}}dx\\
dv=dx\\
v=x\\
x\arctan{x}+\int{\frac{x}{1+x^{2}}\:dx}\\
t=x^{2}+1\\
dt=2xdx\\
x\arctan{x}+\frac{1}{2}\int{\frac{dt}{t}}\\
x\arctan{x}+\frac{1}{2}(\ln{|x^{2}+1|}+C)\\
x\arctan{x}+\frac{1}{2}\ln{|x^{2}+1|}+\frac{1}{2}C
\end{align*}$$