---
date: 29.09.2023
tags:
  - theory
  - differential_equations
---

> [!NOTE] 127
> $2xy'+y=y^{2}\sqrt{x-x^{2}y^{2}}$
> $y=z^{m}\quad y'=mz^{m-1}z'$
> $2mxz^{m-1}z'+z^{m}=z^{2m}\sqrt{x-x^{2}z^{2m}}$
> $1+m-1=m=2m+\frac{1}{2}=2m+1+m$
> $\begin{cases}m=2m+\frac{1}{2}\\ m=3m+1\end{cases}$
> $m=-\frac{1}{2}$
> $2x(-\frac{1}{2}z^{-\frac{3}{2}})+z^{-\frac{1}{2}}=z^{-1}\sqrt{x-x^{2}z^{-1}}$
> $z=tx\quad z'=t'x+t$
> $-\frac{x(t'x+t)}{tx \sqrt{t}\sqrt{x}}+\frac{1}{\sqrt{t}\sqrt{x}}=\frac{1}{tx}\sqrt{x-\frac{x^{2}}{tx}}$
> $-x(t'x+t)+tx=\sqrt{tx^{2}-x^{2}}$
> $z\neq0,\;t\neq0,\;x\neq0$
> $-t'x^{2}=x \sqrt{t-1}\quad(x>0,\;t>0)$
> $-\frac{dt}{dx}=\frac{\sqrt{t-1}}{x}$
> $\frac{dt}{\sqrt{t-1}}+\frac{dx}{x}=0$
> $2\sqrt{t-1}+\ln{x}=C$
> $t=\frac{z}{x}=\frac{1}{xy^{2}}$
> $2\sqrt{\frac{1}{xy^{2}}-1}+\ln{x}=C$
> $y=0$
> $xy^{2}=1\implies y=\frac{1}{\sqrt{x}}$

# Линейные уравнения первого порядка
$y'+\alpha(x)y=\beta(x)$
$x'+\alpha(y)x=\beta(y)$
$y'=\frac{dy}{dx}=\frac{1}{\frac{dx}{dy}}=\frac{1}{x'}$
Метод вариации постоянных
1. $y'+\alpha(x)y=0$ - однородное ДУ 
   $y_{одн}=y(x,c)$
2. $y=y(x, C(x))$ -> в исходное ДУ


> [!example] Пример
> $xy'-2y=2x^{4}$, линейное ДУ 1-го порядка
> 1. $xy'-2y=0$
>    $xdy=2ydx\;|:xy$
>    $\frac{dy}{y}=\frac{2dx}{x}$
>    $\ln{|y|}=2\ln{|x|}+\ln{C}$
>    $y_{одн}=Cx^{2}$
>2. $y=C(x)x^{2}$
>   $y'=C'(x)x^{2}+C(x)2x$
>   $x(C'x^{2}+C2x)-2Cx^{2}=2x^{4}$
>   $C'x^{2}=2x^{4}$
>   $C'=2x$
>   $C=x^{2}+D$
>   $y=(x^{2}+D)x^{2}$

$(2e^{y}-x)y'=1$
$(2e^{y}-x)x'$
$2e^{y}=x'+x$
$\frac{dx}{dy}+x=0$
$\frac{dx}{dy}=-x\quad dy=\frac{dx}{x}$
$y=-\ln{|x|}+C$
$\ln{|x|}=C-y$
$x=e^{C-y}$
$x=\frac{e^{C}}{e^{y}},\;e^C=C_{1}$
$x=\frac{C_{1}}{e^{y}}$
$x=\frac{C(y)}{e^{y}}$
$x'=\frac{C'(y)e^{y}-C(y)e^{y}}{e^{2y}}$
$2e^{y}-\frac{C(y)}{e^{y}}=\frac{C'(y)-C(y)}{e^{y}}$
$2e^{2y}=C'(y)$
$C(y)=e^{2y}+D$
$x=\frac{e^{2y}+D}{e^{y}}$
