а) $y=2x- \frac{3}{x^4}+4\sqrt{x^{3}}$
$y'=2+ \frac{3}{4x^{5}}+12\sqrt{x}$
$y''=\frac{3}{20x^{6}}+6x^{-\frac{1}{2}}$
б) $s=(3-\cos{t})(5+2\sin{t})$
$$\begin{align*}
s'=(3-\cos{t})'(5+2\sin{t})+(3-\cos{t})(5+2\sin{t})'=\\
 \sin{t}(5+2\sin{t})+(3-\cos{t})(2\cos{t})=\\
5\sin{t}+\sin^2{t}+6\cos{t}-2\cos^2{t}
\end{align*}$$
в) $u=\sqrt{V-3\ln{V}}$
$$\begin{align*}
u'=\frac{1}{2}(V-3\ln{V})^{-\frac{1}{2}}(1- \frac{3}{V})
\end{align*}$$
г) $z=\frac{\ln{(4-5t)}}{\sin{t}}$
$$\begin{align*}
z'=\frac{\ln{(4-5t)}'\sin{t}-\ln{(4-5t)}(\sin{t})'}{sin^{2}{t}}=\\
\frac{\frac{\sin{t}}{4-5t}-\ln{(4-5t)}\cos{t}}{\sin^{2}{t}}
\end{align*}$$
---
#practice #mathematical_analysis 