1111-1117
1111. 
$$\begin{align*}
y=x(1+x^{2})^{0.5}\\
y'=(1+x^{2})^{0.5}+x\frac{1}{2(1+x^{2})^{0.5}}2x=(1+x^{2})^{0.5}+x^{2}/(1+x^{2})^{0.5}\\
y''=\frac{x^{2}}{(1+x^{2})^{0.5}}+\frac{2x(1+x^{2})^{0.5}-\frac{x^{3}}{(1+x^{2})^{0.5}}}{1+x^{2}}\\
\end{align*}$$
1113.
$$\begin{align*}
y=e^{-x^{2}}\\
y'=f(g(x))'=f'(g(x))g'(x)\\
y'=(\frac{1}{e^{x^{2}}})'=-e^{(-x^{2})'}\times2x=2xe^{-x^{2}}\\
y''=2e^{-x^{2}}+2x(e^{-x^{2}})=2e^{-x^{2}}+4x^{2}e^{-x^{2}}=2e^{-x^{2}}(1+2x^{2})
\end{align*}$$
1116.
$$\begin{align*}
y=\frac{\arcsin{x}}{(1-x^{2})^{0.5}}\\
y'_{x}=\frac{\frac{1}{(1-x^{2})^{0.5}}(1-x^{2})^{0.5}-\frac{x\arcsin{x}}{(1-x^{2})^{0.5}}}{(1-x^{2})'}=\frac{1}{1-x^{2}}-\frac{\arcsin{x}}{(1-x^{2})^{0.5}}\\
y''=-\frac{1}{(1-x^{2})^{2}}(-2x)-(\frac{1}{(1-x^{2})^{0.5}}(1-x^{2})^{1.5}-\frac{3\arcsin{x}}{2(1-x^{2})^{0.5}})/(1-x^{2})^{3}=\\
=\frac{2x-1}{1-x^{2}}-\frac{3}{2}\frac{\arcsin{x}}{(1-x^{2})^{2.5}}
\end{align*}$$
1123.
$$\begin{align*}
y=(u^{2}+v^{2})^{0.5}\\
y'=\frac{1}{2(u^{2}+v^{2})^{0.5}}((u^{2})'+(v^{2})')=\frac{1}{2(u^{2}+v^{2})^{0.5}}(2u'u+2v'v)\\
y''=-\frac{1}{4}(u^{2}+v^{2})^{-\frac{3}{2}}(2u'u+2v'v)^{2}+\frac{1}{2(u^{2}+v^{2})^{0.5}}(2(u''u+u'^{2})+2(v''v+v'^{2}))=\\
=-\frac{1}{4}\frac{(2u'u+2v'v)^{2}}{(u^{2}+v^{2})^{1.5}}+\frac{u''u+u'^2+v''v+v'^{2}}{(u^{2}+v^{2})^{0.5}}
\end{align*}$$
1156.
$$\begin{align*}
y=x(2x-1)^{2}(x+3)^{3}=x(4x^{2}-4x+1)(x^3+9x^{2}+27x+27)=\\
=(4x^{3}-4x^{2}+x)(x^3+9x^{2}+27x+27)=\\
=4x^{6}+36x^{5}+108x^{4}+108x^{3}+x^{4}+9x^{3}+27x^{2}+27x-4x^{5}-36x^{4}-108x^{3}-108x^{2}=\\
4x^{6}+32x^{5}+73x^{4}+9x^{3}-81x^{2}+27x\\
y'=24x^{5}\quad y''=120x^{4}\quad y'''=480x^{3}\\
...\quad y^{(6)}=2880\quad y^{(7)}=0
\end{align*}$$
1157. Найти $y'''$.
$$\begin{align*}
y=\frac{a}{x^{m}}=ax^{-m}\\
y'=-amx^{-m-1}\\
y''=-am(-m-1)x^{-m-2}=(m+1)amx^{-m-2}\\
y'''=-(m+2)(m+1)amx^{-m-3}\\
y^{(n)}=(-1)^{n}amx^{-(m+n)}\prod\limits_{k=0}^{n}(m+k)
\end{align*}$$
1158. Найти $y^{(10)}$
$$\begin{align*}
y=\sqrt{x}
\end{align*}$$
1190.
$$\begin{align*}
y=\frac{1}{x^{2}-3x+2}=\frac{1}{x-1}-\frac{1}{x-2}\\
y'=-\frac{1}{(x-1)^{2}}+\frac{1}{(x-2)^{2}}\\
y^{(n)}=(-1)^{n}n!(\frac{1}{(x-1)^{n+1}}-\frac{1}{(x-2)^{n+1}})
\end{align*}$$
---
#practice #mathematical_analysis 