$\int{e^{x}\sin{x}dx}$ Первообразную получить проблематично.

$(x^{2})'=2x$
$\int{2x}dx=2\int{x}dx=\frac{2x^{2}}{2}+2c$
$\int{x^{n}}dx=\frac{x^{n+1}}{n+1}+c$

$t=3-x^{2}\implies \sqrt{t-3}=x$
$\int{(3-x^{2})^{3}}dx$
$dt=-2xdx$
$-\frac{dt}{2\sqrt{t-3}}=dx$
$\int{\frac{t^{3}dt}{2\sqrt{t-3}}}=\frac{1}{2}\int{\frac{t^{3}dt}{\sqrt{t-3}}}$

Школьный метод
$\int{(3^{3}-3^{3}x^{2}+3^{2}x^{2}-x^{6})}dx$
$\int{3^{3}}dx-\int{3^{3}x^{2}}dx+\int{3^{2}x^{4}}dx-\int{x^{6}}dx$
$3^{3}\int{}dx-3^{3}\int{x^{2}}dx+3^{2}\int{x^{4}}dx-\int{x^{6}}dx$
$27(x+c_1)-27(\frac{x^{3}}{3}+c_2)+9(\frac{x^{5}}{5}+c_3)-(\frac{x^{7}}{7}+c_4)$
$-\frac{x^{7}}{7}+\frac{9x^{5}}{5}-9x^{3}+27x+c_{5}$, где $c_{5}=27c_{1}-27c_{2}+9c_{3}-c_{4}$

$f'=-x^{6}+9x^{4}-27x^{2}+27$

1629.$$\begin{align*}
\int{x^{2}(5-x)^{4}}dx=\\
\int{x^{2}(625-250x+25x^{2}-250x+100x^{2}-10x^{3}+25x^{2}-10x^{3}+x^{4})}dx=\\
\int{x^{2}(625-500x+150x^{2}-20x^{3}+x^{4})}dx=\\
625\int{x^{2}}dx-500\int{x^{3}}dx+150\int{x^{4}}dx-20\int{x^{5}}dx+\int{x^{6}}dx=\\
625(\frac{x^{3}}{3}+c_1)-500(\frac{x^{4}}{4}+c_2)+150(\frac{x^{5}}{5}+c_3)-20(\frac{x^{6}}{6}+c_4)+\frac{x^{7}}{7}+c_5=\\
\frac{x^{7}}{7}-10\frac{x^{6}}{3}+30x^{5}-125x^4+625\frac{x^{3}}{3}+c_{6}
\end{align*}$$
1631.$$\begin{align*}
\int{\left(\frac{1-x}{x}\right)^{2}}dx=\int{\frac{1}{x^{2}}}dx-2\int{\frac{1}{x}}dx+\int{1}dx=\\
-\frac{1}{x}-c_{1}-2ln|x|-c_{2}+x+c_{3}=-2ln|x|+c_4
\end{align*}$$
1646.$$\begin{align*}
\int{\frac{e^{3x}+1}{e^{x}-1}}dx=\int{\frac{e^{3x}}{e^{x}-1}}dx+\int{\frac{1}{e^{x}-1}}dx=\\
\int{t^{3}(t+1)^{-1}}dx+\int{(t+1)^{-1}}dx=\int{\frac{(m-1)^{3}}{m}}dm\\
\\
\int{\frac{(e^{x}+1)(e^{2x}-e^{x}+1)}{2^{x}+1}}dx=\int{e^{2x}}dx-\int{e^{x}}dx+\int{1}dx=\\
=e^{2x}+c_{1}-e^{x}-c_{2}+x+c_{3}
\end{align*}$$
---
#practice #mathematical_analysis 