[[Определенный интеграл]]
$$\begin{align*}
\int\limits_{0}^{1}{\frac{x^{2}dx}{x^{2}+1}}\\
\int{\frac{x^{2}+1-1}{x^{2}+1}dx}=\int{dx}-\int{\frac{dx}{x^{2}+1}}=x-\arctan{x}+C,\quad C=C_{1}+C_{2}\\
\int\limits_{0}^{1}{\frac{x^{2}dx}{x^{2}+1}}=|_{0}^{1}x-\arctan{x}=1-\frac{\pi}{4}
\end{align*}$$
$$\begin{align*}
\int\limits_{0}^{2}{\frac{x^{3}dx}{\sqrt{x^{4}+4}}}\\
x^{4}+4=t\\
\frac{dt}{4}=x^{3}dx\\
\frac{1}{4}\int\limits_{4}^{20}{\frac{dt}{\sqrt{t}}}=\frac{1}{4}|_{4}^{20}2\sqrt{t}=\frac{1}{4}
\end{align*}$$
$$\begin{align*}
\int\limits_{1}^{2}{\frac{e^{\frac{1}{x}}}{x^{2}}dx}\\
t=\frac{1}{x}\\
dt=-\frac{1}{x^{2}}dx\\
-\int\limits_{1}^{\frac{1}{2}}{e^{t}dt}=-|_{1}^{\frac{1}{2}}e^{t}=e-\sqrt{e}
\end{align*}$$
$$\begin{align*}
\int\limits_{2}^{3}{\frac{x+2}{x^{2}(x-1)}dx}\\
\int\limits_{2}^{3}{\frac{1}{x^{2}}dx}+3\int\limits_{2}^{3}{\frac{1}{x^{2}(x-1)}dx}=|_{2}^{3}\frac{1}{2}\ln{|x^{2}|}+\\

\end{align*}$$
---
#practice #mathematical_analysis 