$$\begin{align*}
\int{\sqrt{e^{2x}-1}\:dx}\\
\int{\sqrt{e^{2x}+a}\:dx}\\
2x=t\quad 2dx=dt\\
\int{\frac{\sqrt{e^{t}+a}}{2}dt}=\frac{1}{2}\int{(e^{t}+a)^{\frac{1}{2}}\:dt}
\end{align*}$$
$$\begin{align*}
\int{\frac{x-3}{(x^{2}-1)(1+2x)}dx}\\
\frac{x-3}{(x+1)(x-1)(1+2x)}=\frac{A}{x+1}+\frac{B}{x-1}+\frac{C}{1+2x}\\
A(x-1)(1+2x)+B(x+1)(2x+1)+C(x^{2}-1)=x-3\\
3B=-1\\
A=-2\\
-\frac{3}{2}C=-7\\
-2\int{\frac{dx}{x+1}}-\frac{1}{3}\int{\frac{dx}{x-1}}+\frac{14}{3}\int{\frac{dx}{1+2x}}
\end{align*}$$
$$\begin{align*}
\int{\frac{\sqrt[3]{x}}{2x+1}dx}\\
x=t^{3}\\
dx=3t^{2}dt\\
\int{\frac{3t}{2t^{3}+1}dt}=3\int{\frac{t}{(\sqrt[3]{2}t+1)(2^\frac{2}{3}t^2-2^\frac{1}{3}t+1)}}\\
\frac{t}{(\sqrt[3]{2}t+1)(2^{\frac{2}{3}}t^{2}-2^{\frac{1}{3}}t+1)}=\frac{A}{\sqrt[3]{2}t+1}+\frac{Bt+C}{2^{\frac{2}{3}}t^{2}-2^{\frac{1}{3}}t+1}
\end{align*}$$
---
#homework #mathematical_analysis 